Started sketching 2pc invariant

src/program_proof/lockservice/two_pc_example.v
@@ -10,6 +10,8 @@ Section tpc_example.
 
 Context `{!heapG Σ}.
 Context `{!mapG Σ u64 u64}.
+Context `{!mapG Σ u64 (option bool)}.
+Context `{!mapG Σ (u64*u64) ()}.
 
 Record participant_names :=
 mk_participant_names  {
@@ -19,16 +21,23 @@ mk_participant_names  {
 
 Record tpc_names :=
 mk_tpc_names  {
+  committed_gn : gname ; (* tid -> option bool *)
+  prepared_gn : gname ;  (* (tid, pid) -> () *)
 }.
 
 Implicit Type γtpc : tpc_names.
 Implicit Type γ : participant_names.
 
-Definition tpc_inv : iProp Σ := True.
+Definition prepared γtpc (tid pid:u64) : iProp Σ := (tid, pid)[[γtpc.(prepared_gn)]]↦ro ().
 
-Definition is_txn (tid:u64) γtpc : iProp Σ := True.
+Definition tpc_inv γtpc tid R0 R1 : iProp Σ :=
+  (tid [[γtpc.(committed_gn)]]↦ None ∗
+   (prepared γtpc tid 0 ∨ R0) ∗
+   (prepared γtpc tid 1 ∨ R1)) ∨
+  ∃ d, tid [[γtpc.(committed_gn)]]↦ Some d.
 
-Definition prepared γtpc (tid:u64) : iProp Σ := True.
+Definition tpcN := nroot .@ "tpc".
+Definition is_txn (tid:u64) γtpc R0 R1 : iProp Σ := inv tpcN (tpc_inv γtpc tid R0 R1).
 
 Record TransactionC :=
 mkTransactionC {
@@ -54,33 +63,35 @@ Proof.
   done.
 Defined.
 
-Definition ps_mu_inv (ps:loc) γ γtpc : iProp Σ :=
+Definition ps_mu_inv (ps:loc) γ γtpc pid : iProp Σ :=
   ∃ (kvs_ptr txns_ptr lockMap_ptr:loc) (kvsM:gmap u64 u64) (txnsM:gmap u64 TransactionC),
     "Hkvs" ∷ ps ↦[ParticipantServer.S :: "kvs"] #kvs_ptr ∗
     "Htxns" ∷ ps ↦[ParticipantServer.S :: "txns"] #txns_ptr ∗
+    "HlockMap_ptr" ∷ ps ↦[ParticipantServer.S :: "lockmap"] #lockMap_ptr ∗
     "HkvsMap" ∷ is_map (kvs_ptr) kvsM ∗
     "HtxnsMap" ∷ is_map (txns_ptr) txnsM ∗
     "Hkvs_ctx" ∷ map_ctx γ.(ps_kvs) 1 kvsM ∗
-    "HlockMap" ∷ is_lockMap lockMap_ptr γ.(ps_ghs) (fin_to_set u64) (λ x, x [[γ.(ps_kvs)]]↦{1/2} (map_get kvsM x).1) ∗
-    "Htxnx_prepared" ∷ [∗ map] tid ↦ txn ∈ txnsM, (prepared γtpc tid)
+    "#HlockMap" ∷ is_lockMap lockMap_ptr γ.(ps_ghs) (fin_to_set u64) (λ x, x [[γ.(ps_kvs)]]↦{1/2} (map_get kvsM x).1) ∗
+    "Htxnx_prepared" ∷ [∗ map] tid ↦ txn ∈ txnsM, (prepared γtpc tid pid)
 .
 
 Definition participantN := nroot .@ "participant".
 
-Definition is_participant (ps:loc) γ γtpc : iProp Σ :=
+Definition is_participant (ps:loc) γ γtpc pid : iProp Σ :=
   ∃ (mu:loc),
   "#Hmu" ∷ readonly (ps ↦[ParticipantServer.S :: "mu"] #mu) ∗
-  "#Hmu_inv" ∷ is_lock participantN #mu (ps_mu_inv ps γ γtpc)
+  "#Hmu_inv" ∷ is_lock participantN #mu (ps_mu_inv ps γ γtpc pid)
 .
 
-Lemma wp_PrepareIncrease (ps:loc) tid γ γtpc key amnt :
+(* TODO: One participant shouldn't know the resources that other participants are contributing *)
+Lemma wp_PrepareIncrease (ps:loc) tid γ γtpc (key key' amnt:u64) :
   {{{
-       is_txn tid γtpc ∗
-       is_participant ps γ γtpc
+       is_txn tid γtpc (∃ v:u64, key [[γ.(ps_kvs)]]↦{1/2} v) (∃ v:u64, key' [[γ.(ps_kvs)]]↦{1/2} v) ∗
+       is_participant ps γ γtpc 0
   }}}
     ParticipantServer__PrepareIncrease #ps #tid #key #amnt
   {{{
-       (a:u64), RET #a; ⌜a ≠ 0⌝ ∨ ⌜a = 0⌝ ∗ prepared γtpc tid
+       (a:u64), RET #a; ⌜a ≠ 0⌝ ∨ ⌜a = 0⌝ ∗ prepared γtpc tid 0
   }}}.
 Proof.
   iIntros (Φ) "[#Htxn #Hps] HΦ".
@@ -101,6 +112,59 @@ Proof.
     (* Use Htxns_prepared *)
     admit.
   }
+  wp_loadField.
+  wp_apply (wp_LockMap__Acquire with "[$HlockMap]").
+  { iPureIntro. set_solver. }
+  iIntros "[Hptsto Hkeylocked]".
+  wp_pures.
+  wp_loadField.
+  wp_apply (wp_MapGet with "HkvsMap").
+  iIntros (old_v old_v_ok) "[%Hmapget_v HkvsMap]".
+  wp_pures.
+  wp_loadField.
+  wp_apply (wp_MapInsert _ _ _ _ (mkTransactionC _ _ _ _) with "HtxnsMap").
+  { eauto. }
+  iIntros "HtxnsMap".
+  wp_pures.
+  wp_loadField.
+  wp_apply (wp_MapGet with "HkvsMap").
+  iIntros (old_v' ok') "[Hmapget_oldv' HkvsMap]".
+  wp_pures.
+  wp_loadField.
+  wp_apply (wp_MapInsert with "HkvsMap").
+  { eauto. }
+  iIntros "HkvsMap".
+  iApply wp_fupd.
+  wp_pures.
+  iApply "HΦ".
+
+  (* FIXME: lock release missing *)
+
+  (* Get prepared token *)
+  iInv "Htxn" as ">Ht" "Htclose".
+  iDestruct "Ht" as "[Ht|Ht]".
+  {
+    iDestruct "Ht" as "(Hundecided & [Hprep | Hptsto2] & Hirrelevant)"; last first.
+    {
+      iNamed "Hptsto2".
+      (* TODO: Need to add token to rule out this case *)
+      admit.
+    }
+    iMod ("Htclose" with "[Hirrelevant Hptsto Hundecided]") as "_".
+    {
+      iNext.
+      iLeft.
+      iFrame. iRight.
+      iExists _; iFrame.
+    }
+    iModIntro.
+    iRight.
+    iFrame. done.
+  }
+  { (* Impossible case; commit already decided *)
+    admit.
+  }
+
 Admitted.
 
 End tpc_example.
